# Section 5.3 L'Hospital's Rule

### **1. Infinite Limits (Definitions)**
Before introducing L'Hospital's rule, formal definitions for infinite limits are established to handle the indeterminate form $\infty/\infty$.

* **Definition 5.3.1:** Let $f$ be defined on a subset $E \subset \mathbb{R}$ and $p$ be a limit point of $E$.
    * $\lim_{x \to p} f(x) = \infty$ if for every $M \in \mathbb{R}$, there exists $\delta > 0$ such that $f(x) > M$ for all $x \in E$ with $0 < |x - p| < \delta$.
    * $\lim_{x \to p} f(x) = -\infty$ is defined similarly (where $f(x) < M$).
* **Note:** These definitions extend to limits at infinity ($\lim_{x \to \infty}$) and one-sided limits ($\lim_{x \to p^+}$).

---

### **2. L'Hospital's Rule (Theorem 5.3.2)**
This rule evaluates limits of indeterminate forms $0/0$ or $\infty/\infty$.

**Hypotheses:**
1.  $f, g$ are real-valued differentiable functions on $(a, b)$.
2.  $g'(x) \neq 0$ for all $x \in (a, b)$.
3.  $\lim_{x \to a^+} \frac{f'(x)}{g'(x)} = L$, where $L \in \mathbb{R} \cup \{-\infty, \infty\}$.

**Conditions (Indeterminate Forms):**
* **(a) Case $0/0$:** $\lim_{x \to a^+} f(x) = 0$ and $\lim_{x \to a^+} g(x) = 0$.
* **(b) Case $\infty/\infty$:** $\lim_{x \to a^+} g(x) = \pm \infty$ (Note: $f(x)$ does not strictly need to tend to $\infty$, but usually does).

**Conclusion:**
$$\lim_{x \to a^+} \frac{f(x)}{g(x)} = L$$
*(Note: The rule applies equally to $x \to b^-$, $x \to p$, or $x \to \pm \infty$).*

---

### **3. Proofs: Core Ideas**

#### **Case A: Indeterminate Form $0/0$ (Finite $a$)**
* **Key Tool:** Generalized Mean Value Theorem (GMVT).
* **Method:**
    1.  Since we are dealing with limits approaching $a$, we define $f(a) = g(a) = 0$ to make the functions continuous at $a$.
    2.  Consider a sequence $\{x_n\} \to a^+$. Apply GMVT on the interval $[a, x_n]$.
    3.  There exists $c_n$ between $a$ and $x_n$ such that:
        $$\frac{f(x_n) - f(a)}{g(x_n) - g(a)} = \frac{f'(c_n)}{g'(c_n)}$$
    4.  Since $f(a)=g(a)=0$, this simplifies to $\frac{f(x_n)}{g(x_n)} = \frac{f'(c_n)}{g'(c_n)}$.
    5.  As $n \to \infty$, $x_n \to a$ implies $c_n \to a$. Therefore, the limit of the ratio of functions equals the limit of the ratio of derivatives.

#### **Case B: Limits at Infinity ($x \to -\infty$)**
* **Key Tool:** Substitution.
* **Method:** Let $x = -1/t$. As $t \to 0^+$, $x \to -\infty$.
    * Define $\phi(t) = f(-1/t)$ and $\psi(t) = g(-1/t)$.
    * Using chain rule differentiation, the problem reduces to a limit at $0^+$, which allows the use of the previous proof logic.

#### **Case C: Indeterminate Form $\infty/\infty$**

* **Key Tool:** GMVT + Bounding Argument (No need for $f, g$ to be continuous at $a$).
* **Method:**
    1.  Assume $\lim \frac{f'(x)}{g'(x)} = L$.
    2.  Fix $y$ and let $x$ vary. Apply GMVT on interval $(x, y)$ to get $\frac{f(x)-f(y)}{g(x)-g(y)} = \frac{f'(\zeta)}{g'(\zeta)}$.
    3.  **Algebraically rearrange** the GMVT equation to isolate $\frac{f(x)}{g(x)}$:
        $$\frac{f(x)}{g(x)} = \frac{f'(\zeta)}{g'(\zeta)} \left( 1 - \frac{g(y)}{g(x)} \right) + \frac{f(y)}{g(x)}$$
    4.  Since $g(x) \to \infty$ as $x \to a^+$, the term $\frac{g(y)}{g(x)} \to 0$ and $\frac{f(y)}{g(x)} \to 0$.
    5.  This implies that for $x$ sufficiently close to $a$, $\frac{f(x)}{g(x)}$ becomes arbitrarily close to $\frac{f'(\zeta)}{g'(\zeta)} \cdot (1 - 0) + 0$, which converges to $L$.
---

### **4. Examples**

#### **(a) Basic Application ($0/0$)**
**Problem:** Compute $\lim_{x \to 0^+} \frac{\ln(1+x)}{x}$.
* **Form:** $0/0$ (since $\ln(1)=0$).
* **Apply L'Hospital's:**
    $$\lim_{x \to 0^+} \frac{\frac{d}{dx}\ln(1+x)}{\frac{d}{dx}x} = \lim_{x \to 0^+} \frac{\frac{1}{1+x}}{1} = 1$$
* **Note:** This can also be proven using inequalities derived from the Taylor expansion or Mean Value Theorem (i.e., $\frac{x}{1+x} \leq \ln(1+x) \leq x$), but L'Hospital's is more direct.

#### **(b) Repeated Application**
**Problem:** Compute $\lim_{x \to 0} \frac{1 - \cos x}{x^2}$.
* **Form:** $0/0$.
* **First Application:**
    $$\lim_{x \to 0} \frac{\sin x}{2x}$$
    This is *still* form $0/0$.
* **Second Application:**
    $$\lim_{x \to 0} \frac{\cos x}{2} = \frac{1}{2}$$
* **Result:** The limit is $1/2$.

#### **(c) Importance of Substitution (Avoiding Complexity)**
**Problem:** Compute $\lim_{x \to 0^+} \frac{e^{-1/x}}{x}$.
* **Form:** $0/0$ (since $e^{-\infty} \to 0$).
* **Direct L'Hospital's Failure:** Differentiating directly gives $\frac{e^{-1/x} \cdot (1/x^2)}{1}$, which simplifies to $\frac{e^{-1/x}}{x^2}$. This is *more* complicated than the original.
* **Correct Approach:** Use substitution $t = 1/x$. As $x \to 0^+$, $t \to \infty$.
    $$\lim_{t \to \infty} \frac{t}{e^t}$$
* **New Form:** $\infty/\infty$.
* **Apply L'Hospital's:**
    $$\lim_{t \to \infty} \frac{1}{e^t} = 0$$
* **Result:** The original limit is 0.