# **Chapter 5.1: The Derivative**

### **1. Definition of the Derivative**

**Historical Context:** Formulated rigorously by Cauchy (1821) using limits, moving away from vague notions of tangent lines and velocity.

**Definition 5.1.1 (The Derivative)**
Let $I \subset \mathbb{R}$ be an interval and $f: I \to \mathbb{R}$. For a fixed $p \in I$, the derivative $f'(p)$ is:
$$f'(p) = \lim_{x \to p} \frac{f(x) - f(p)}{x - p}$$
Alternatively, letting $x = p+h$:
$$f'(p) = \lim_{h \to 0} \frac{f(p+h) - f(p)}{h}$$
* **Geometric interpretation:** Slope of the tangent line at $(p, f(p))$.
* **Physical interpretation:** Instantaneous velocity.

---

### **2. One-Sided Derivatives**

If $p$ is an endpoint or we need to analyze corner points, we use one-sided limits (Definition 5.1.2).

* **Right Derivative ($f'_+(p)$):** $\displaystyle \lim_{h \to 0^+} \frac{f(p+h) - f(p)}{h}$
* **Left Derivative ($f'_-(p)$):** $\displaystyle \lim_{h \to 0^-} \frac{f(p+h) - f(p)}{h}$

**Key Property:**
For an interior point $p \in I$, $f'(p)$ exists **if and only if** both $f'_+(p)$ and $f'_-(p)$ exist and are **equal**.

---

### **3. Worked Examples (Specific Functions)**

The text analyzes the differentiability of several specific functions to illustrate the definition.

**A. Power Function ($f(x) = x^2$)**
$$f'(x) = \lim_{h \to 0} \frac{(x+h)^2 - x^2}{h} = \lim_{h \to 0} (2x + h) = 2x$$
*(Note: Generalizes to $f(x)=x^n \implies f'(x) = nx^{n-1}$)*.

**B. Square Root ($f(x) = \sqrt{x}, x > 0$)**
Uses rationalization:
$$\frac{\sqrt{x+h} - \sqrt{x}}{h} = \frac{1}{\sqrt{x+h} + \sqrt{x}} \xrightarrow{h \to 0} \frac{1}{2\sqrt{x}}$$

**C. Sine Function ($f(x) = \sin x$)**
Uses the identity $\sin(x+h) = \sin x \cos h + \cos x \sin h$:
$$\frac{\sin(x+h) - \sin x}{h} = \sin x \left(\frac{\cos h - 1}{h}\right) + \cos x \left(\frac{\sin h}{h}\right)$$
Since $\lim_{h \to 0} \frac{\sin h}{h} = 1$ and $\lim_{h \to 0} \frac{\cos h - 1}{h} = 0$, $f'(x) = \cos x$.

**D. Absolute Value ($f(x) = |x|$) at $x=0$**
* $f'_+(0) = \lim_{h \to 0^+} \frac{h}{h} = 1$
* $f'_-(0) = \lim_{h \to 0^-} \frac{-h}{h} = -1$
* **Result:** $f'_+(0) \neq f'_-(0)$, so $f$ is **not differentiable** at $0$.

**E. Cusp ($g(x) = x^{3/2}$) at $x=0$**
$$g'(0) = \lim_{h \to 0^+} \frac{h^{3/2}}{h} = \lim_{h \to 0^+} \sqrt{h} = 0$$
Differentiable at 0.

**F. Oscillating Discontinuity ($f(x) = x \sin(1/x)$ for $x \neq 0$, $f(0)=0$)**
$$f'(0) = \lim_{h \to 0} \frac{h \sin(1/h) - 0}{h} = \lim_{h \to 0} \sin\left(\frac{1}{h}\right)$$
**Result:** Limit does not exist. Not differentiable at 0.

**G. Differentiable with Discontinuous Derivative ($g(x) = x^2 \sin(1/x)$ for $x \neq 0$, $g(0)=0$)**
* **At $x=0$:**
    $$g'(0) = \lim_{h \to 0} \frac{h^2 \sin(1/h)}{h} = \lim_{h \to 0} h \sin\left(\frac{1}{h}\right) = 0$$
    (By Squeeze Theorem).
* **For $x \neq 0$:** $g'(x) = 2x \sin(1/x) - \cos(1/x)$.
* **Observation:** $\lim_{x \to 0} g'(x)$ does not exist (due to $\cos(1/x)$).
* **Conclusion:** $g$ is differentiable everywhere, but $g'$ is **not continuous** at 0.

---

### **4. Relationship between Differentiability and Continuity**

**Theorem 5.1.4:**
If $f$ is differentiable at $p$, then $f$ is continuous at $p$.

**Proof Sketch:**
$$\lim_{t \to p} (f(t) - f(p)) = \lim_{t \to p} \left[ \frac{f(t)-f(p)}{t-p} \cdot (t-p) \right] = f'(p) \cdot 0 = 0$$
Thus $\lim_{t \to p} f(t) = f(p)$.

* **Converse:** False. Continuity does **not** imply differentiability (e.g., $f(x)=|x|$).
* **Weierstrass Function:** An example of a function continuous everywhere but differentiable nowhere.

---

### 5. Arithmetic of Derivatives

**Theorem 5.1.5 (Algebraic Rules)**
Let $f, g$ be differentiable at $x$.

#### A. Sum Rule
$$(f+g)'(x) = f'(x) + g'(x)$$

#### B. Product Rule
$$(fg)'(x) = f'(x)g(x) + f(x)g'(x)$$

**Key Proof Idea: The "Add and Subtract" Trick**
Direct substitution creates a mixed term $f(x+h)g(x+h)$ that cannot be factored. To fix this, we insert a "middle term" into the numerator.

**Proof Sketch:**
1.  **Setup:** Start with the difference quotient:
    $$\frac{f(x+h)g(x+h) - f(x)g(x)}{h}$$
2.  **The Trick:** Add and subtract **$f(x+h)g(x)$**:
    $$\frac{f(x+h)g(x+h) \mathbf{- f(x+h)g(x) + f(x+h)g(x)} - f(x)g(x)}{h}$$
3.  **Group & Limit:** Separate into two parts:
    $$f(x+h) \underbrace{\left[ \frac{g(x+h) - g(x)}{h} \right]}_{\to g'(x)} + g(x) \underbrace{\left[ \frac{f(x+h) - f(x)}{h} \right]}_{\to f'(x)}$$
    *Note: $f(x+h) \to f(x)$ because differentiability implies continuity.*

---

#### C. Quotient Rule (Reciprocal Case)
To prove the quotient rule, we first focus on the derivative of the reciprocal.

**The Reciprocal Rule:**
$$\left(\frac{1}{g}\right)'(x) = -\frac{g'(x)}{[g(x)]^2}$$

**Proof Sketch:**
1.  **Common Denominator:**
    $$\frac{\frac{1}{g(x+h)} - \frac{1}{g(x)}}{h} = \frac{g(x) - g(x+h)}{h \cdot g(x+h)g(x)}$$
2.  **Extract Derivative Definition:**
    Recognize that $g(x) - g(x+h) = -[g(x+h) - g(x)]$:
    $$-\underbrace{\left[ \frac{g(x+h) - g(x)}{h} \right]}_{\to g'(x)} \cdot \frac{1}{g(x+h)g(x)}$$
3.  **Take Limit ($h \to 0$):**
    Since $g$ is continuous, $g(x+h) \to g(x)$, giving the denominator $[g(x)]^2$.

*(Note: The full Quotient Rule is simply the Product Rule applied to $f(x) \cdot [1/g(x)]$.)*


---

### **6. The Chain Rule**

**Theorem 5.1.6 (Composition)**
If $f$ is differentiable at $x$ and $g$ is differentiable at $y = f(x)$, then $h = g \circ f$ is differentiable at $x$:
$$h'(x) = g'(f(x)) \cdot f'(x)$$


**Proof:** Linear Approximation (to avoid division by zero).

Standard limits fail if $f(t)-f(x)=0$. Instead, use "error terms" ($u, v$) that go to 0:
*  **$f$:** $f(t) - f(x) = (t-x)[f'(x) + u(t)]$
*  **$g$:** $g(s) - g(y) = (s-y)[g'(y) + v(s)]$
*  Set $s=f(t)$ and $y=f(x)$. The difference quotient becomes:
    $$\frac{g(f(t)) - g(f(x))}{t-x} = [f'(x) + u(t)] \cdot [g'(y) + v(f(t))]$$
* As $t \to x$, the error terms vanish ($u, v \to 0$), leaving $f'(x)g'(y)$.

**Examples:**
* **Composite Trig:** $h(x) = \sin(1/x^2)$.
    $$h'(x) = \cos\left(\frac{1}{x^2}\right) \cdot \frac{d}{dx}(x^{-2}) = \cos\left(\frac{1}{x^2}\right) \cdot (-2x^{-3})$$
* **Power Rule Extension:** $\frac{d}{dx}[f(x)]^n = n[f(x)]^{n-1}f'(x)$.












